LF to Hyb contexts

LanguagesEquivalence/LF_to_Hyb.v
@@ -6,11 +6,92 @@ Require Import Shared.
 Require Import LabelFree.
 Require Import Hybrid.
 Require Import Arith.
+Require Import ListLib.
 
 Open Scope is5_scope.
 Open Scope permut_scope.
 (* FIXME: There is no labelfree is5 scope *)
 Open Scope hybrid_is5_scope.
+
+Fixpoint LF_to_Hyb_ctx (G: bg_LF) (U: list var) : bg_Hyb :=
+match G with
+| nil => nil
+| Gamma::G' =>
+  let w := var_gen (from_list U) in
+  (w, Gamma) :: (LF_to_Hyb_ctx G' (w::U))
+end.
+
+Lemma LF_to_Hyb_ctx_Ok_simpl1:
+forall G X U,
+  ok_LF (X ++ concat G) U -> ok_Hyb (LF_to_Hyb_ctx G (map fst_ X ++ U)) U.
+induction G; simpl; intros; rew_concat in *; [constructor | ].
+constructor. apply notin_Mem; subst; apply var_gen_spec.
+apply IHG with (X:=X++a); rew_app.
+apply ok_LF_fresh_used; auto.
+apply notin_Mem; rew_app.
+
+
+Lemma LF_to_Hyb_ctx_Ok:
+forall G,
+  ok_Bg_LF G -> ok_Bg_Hyb (LF_to_Hyb_ctx G nil).
+unfold ok_Bg_LF in *; intros;
+eapply LF_to_Hyb_ctx_Ok_simpl; eauto.
+Qed.
+
+Inductive LF_to_Hyb_term: vwo -> te_LF -> te_Hyb -> Prop :=
+| hyp_LF_Hyb:
+    forall v w, LF_to_Hyb_term w (hyp_LF v) (hyp_Hyb v)
+| lam_LF_Hyb:
+    forall L M N t w,
+      (forall v0, v0 \notin L ->
+                  LF_to_Hyb_term w
+                    (open_LF M (hyp_LF (fte v0)))
+                    (open_t_Hyb N (hyp_Hyb (fte v0)))) ->
+      LF_to_Hyb_term w (lam_LF t M) (lam_Hyb t N)
+| appl_LF_Hyb:
+    forall M M' N N' w,
+      LF_to_Hyb_term w M M' ->
+      LF_to_Hyb_term w N N' ->
+      LF_to_Hyb_term w (appl_LF M N) (appl_Hyb M' N')
+| box_LF_Hyb:
+    forall L M N w,
+      (forall w0, w0 \notin L -> LF_to_Hyb_term w0 M (open_w_Hyb N w0)) ->
+      LF_to_Hyb_term w (box_LF M) (box_Hyb N)
+| unbox_LF_Hyb:
+    forall M N w w',
+      LF_to_Hyb_term w M N ->
+      LF_to_Hyb_term w' (unbox_LF M) (unbox_fetch_Hyb w N)
+| here_LF_Hyb:
+    forall M N w w',
+      LF_to_Hyb_term w M N ->
+      LF_to_Hyb_term w' (here_LF M) (get_here_Hyb w N)
+| letdia_LF_Hyb:
+    forall M M' N N' w w',
+      LF_to_Hyb_term w M M' ->
+      LF_to_Hyb_term w' N N' ->
+      LF_to_Hyb_term w' (letdia_LF M N) (letdia_get_Hyb w M' N')
+.
+
+Lemma LF_to_Hyb_typing:
+forall G0 Gamma0 M0 A G w M,
+  LF_to_Hyb_ctx (Gamma0::G0) \{} = (w, Gamma0) :: G ->
+  LF_to_Hyb_term (fwo w) M0 M ->
+  types_LF G0 Gamma0 M0 A ->
+  G |= (w, Gamma0) |- M ::: A.
+intros; induction H1; inversion H0; subst.
+constructor.
+
+Lemma LF_to_Hyb_steps:
+forall M M' N,
+  steps_LF M M' ->
+  LF_to_Hyb_term M N ->
+  exists N',
+    steps_Hyb N N' /\ LF_to_Hyb_term M' N'.
+
+Lemma LF_to_Hyb_left_total:
+forall M, exists N,
+  LF_to_Hyb_term M N.
+
 
 Close Scope hybrid_is5_scope.
 Close Scope permut_scope.
